theories/ordinals/Ackermann/model.v
@@ -1,12 +1,16 @@
-Require Import Ensembles.
-Require Import Coq.Lists.List.
+(** model.v :
+
+   Original script by Russel O'Connor
+*)
+
+
+From Coq Require Import Ensembles List Vector Arith.
+
 Require Import ListExt.
 Require Import folProof.
 Require Import folProp.
-Require Vector.
 Require Import Peano_dec.
 Require Import misc.
-Require Import Arith.
 Require Import NewNotations.
 
 Section Model_Theory.
@@ -72,13 +76,13 @@ Fixpoint interpFormula (value : nat -> U M) (f : Formula L) {struct f} :
   end.
 
 Lemma freeVarInterpTerm (v1 v2 : nat -> U M) (t : Term L):
- (forall x : nat, In x (freeVarTerm L t) -> v1 x = v2 x) ->
+ (forall x : nat, List.In x (freeVarTerm L t) -> v1 x = v2 x) ->
  interpTerm v1 t = interpTerm v2 t.
 Proof.
   elim t using  Term_Terms_ind with
     (P0 := fun (n : nat) (ts : Terms L n) =>
              forall f : naryFunc (U M) n,
-               (forall x : nat, In x (freeVarTerms L n ts) -> v1 x = v2 x) ->
+               (forall x : nat, List.In x (freeVarTerms L n ts) -> v1 x = v2 x) ->
                interpTerms n f v1 ts = interpTerms n f v2 ts); 
     simpl.
   - intros n H; apply H; left; auto.
@@ -98,7 +102,7 @@ Qed.
 
 Lemma freeVarInterpRel (v1 v2 : nat -> U M) (n : nat) 
   (ts : Terms L n) (r : naryRel (U M) n): 
-  (forall x : nat, In x (freeVarTerms L n ts) -> v1 x = v2 x) ->
+  (forall x : nat, List.In x (freeVarTerms L n ts) -> v1 x = v2 x) ->
   interpRels n r v1 ts -> interpRels n r v2 ts.
 Proof.
   intros H; induction ts as [| n t ts Hrects]; simpl in |- *.
@@ -112,7 +116,7 @@ Proof.
 Qed.
 
 Lemma freeVarInterpFormula (v1 v2 : nat -> U M) (g : Formula L):
- (forall x : nat, In x (freeVarFormula L g) -> v1 x = v2 x) ->
+ (forall x : nat, List.In x (freeVarFormula L g) -> v1 x = v2 x) ->
  interpFormula v1 g -> interpFormula v2 g.
 Proof.
   revert v1 v2.
@@ -233,12 +237,12 @@ Proof.
     + induction (In_dec eq_nat_dec v (freeVarTerm L s)) as [a0 | b0].
       * simpl;
         set (nv := newVar (v0 :: freeVarTerm L s ++ freeVarFormula L a)) in *.
-        assert (~ In nv (v0 :: freeVarTerm L s ++ freeVarFormula L a)).
+        assert (~ List.In nv (v0 :: freeVarTerm L s ++ freeVarFormula L a)).
         { unfold nv in |- *.
           apply newVar1. }
         assert
               (forall (x : U M) (x0 : nat),
-                  In x0 (freeVarFormula L a) ->
+                  List.In x0 (freeVarFormula L a) ->
                   updateValue (updateValue value v0 (interpTerm value s)) v x x0 =
                     updateValue
                       (updateValue (updateValue value nv x) v0
@@ -357,7 +361,7 @@ Proof.
       * simpl in |- *.
         assert
           (forall (x : U M) (x0 : nat),
-              In x0 (freeVarFormula L a) ->
+              List.In x0 (freeVarFormula L a) ->
               updateValue (updateValue value v0 (interpTerm value s)) v x x0 =
                 updateValue (updateValue value v x) v0
                   (interpTerm (updateValue value v x) s) x0).
@@ -489,7 +493,7 @@ Proof.
   intros H g H0.
   induction H0 as (x, H0).
   induction H0 as (x0, H0).
-  cut (forall g : Formula L, In g x -> interpFormula value (nnTranslate g)).
+  cut (forall g : Formula L, List.In g x -> interpFormula value (nnTranslate g)).
   - clear H H0; revert value.
     induction x0
       as
